src/Concurrent/Experimental/BisimReductions.v
@@ -3320,3 +3320,96 @@ Theorem normalise_common :
 
 
 
+
+(* 
+Lemma bisim_congr :
+  forall U Π Π' eth eth', (eth, Π) ~ (eth', Π') using U ->
+    forall Π2, (eth, Π ∪ Π2) ~ (eth', Π' ∪ Π2) using U.
+Proof.
+  cofix IH. intros. inv H. constructor; auto; simpl in *.
+  * clear -H0. destruct H0. split; unfold preCompatibleNodes in *; intros.
+    - apply isUntaken_comp in H1 as [H1_1 H1_2].
+      apply H in H1_1.
+      assert (isUntaken ι (eth', Π2)). {
+        destruct H1_1, H1_2. split; auto.
+      }
+      now apply isUntaken_comp.
+    - apply isUntaken_comp in H1 as [H1_1 H1_2].
+      apply H0 in H1_1.
+      assert (isUntaken ι (eth, Π2)). {
+        destruct H1_1, H1_2. split; auto.
+      }
+      now apply isUntaken_comp.
+  * clear H4 H5 H6. intros. destruct A'.
+    apply step_in_comp in H as H'. destruct H' as [[Π1' [? ?]] | [Π2' [? ?]]].
+    - subst. apply H3 in H4 as H4'. destruct_hyps. destruct x as [e' Π1''].
+      (* (* At this point, we need renamings :( - or to know what PIDs are
+         spawned by Π *)
+      Print reductionPreCompatibility.
+      (* spawns in x0 should be distinct from:
+         - syntactically used PIDs in Π2 - for goal 3
+         - ι0 -> if a = send(ι, ι0 <- destination, msg)
+         - We also need a proof that (eth, Π) ~ (eth[x|->y], Π[x|->y])
+      *)
+      exists (e', Π1'' ∪ Π2), x0. split. 2: split. 3: split.
+      4: { apply IH. assumption. }
+      3: apply reductions_are_preserved_by_comp; auto.
+      3: {
+        intros. destruct H6 as [H6 _]. rewrite Forall_forall in H6.
+        apply H6 in H9. unfold isUntaken in H9. simpl in *.
+      } *)
+      admit.
+    - subst. exists (e, Π' ∪ Π2'), [(a, ι)]. split_and!.
+      + split.
+        ** destruct a; auto. simpl. constructor; auto. intro.
+           eapply (no_spawn_unTaken (eth, Π ∪ Π2)). eapply n_trans. eassumption.
+           apply n_refl. 2: cbn; left; reflexivity.
+           apply isUntaken_comp in H5 as [? ?]. apply H0 in H5.
+           apply isUntaken_comp; split; auto.
+           (* ι0 should be Untaken wrt. eth *)
+           destruct H5, H6. split; simpl in *; auto.
+        ** intros; simpl in *; destruct a; auto; simpl in *.
+           destruct_or!; auto. split. 2: split; auto.
+           subst.
+           (* ISSUE: we do not know, whether Π' uses ι0 *)
+           (* is it okay to assume, that Π2 does not communicate to 
+              PIDs in the domain of Π/Π' -> NO!
+
+              is it okay to assume, that Π2 does not communicate to
+              PIDs in ((dom Π ∪ dom Π') \ (dom Π ∩ dom Π')). Probably not.
+            *)
+           admit.
+      + split.
+        ** destruct a; auto. simpl. constructor; auto. intro.
+           eapply (no_spawn_unTaken (eth, Π ∪ Π2)). eapply n_trans. eassumption.
+           apply n_refl. 2: cbn; left; reflexivity.
+           apply isUntaken_comp in H5 as [? ?].
+           apply isUntaken_comp; split; auto.
+        ** intros; simpl in *; destruct a; auto; simpl in *.
+           destruct_or!; auto. split. 2: split; auto.
+           subst.
+           (* ISSUE: we do not know, whether Π uses ι0
+              BOTTOMLINE: we should specify where can Π2 send messages?
+            *)
+           admit.
+      + econstructor.
+        apply reduction_is_preserved_by_comp_r. (* eassumption. *) admit. admit. admit. admit.
+      + admit.
+(*     - subst. exists (e, Π ∪ Π2'), [(a, ι)]. split_and!.
+      split.
+      + destruct a; auto. simpl. constructor; auto. intro.
+        eapply (no_spawn_unTaken (eth, Π ∪ Π2)). eapply n_trans. eassumption.
+        apply n_refl. 2: cbn; left; reflexivity.
+        apply isUntaken_comp in H5 as [? ?]. apply H0 in H5.
+        apply isUntaken_comp; split; auto.
+        (* ι0 should be Untaken wrt. eth *)
+        destruct H5, H6. split; simpl in *; auto.
+      + intros; simpl in *; destruct a; auto; simpl in *.
+        destruct_or!; auto. split. 2: split; auto.
+        subst.
+        (* ISSUE: we do not know, whether Π' uses ι0 *)
+        admit.
+      4: { apply IH. apply barbedBisim_refl. } *)
+Abort.
+ *)
+
